mload and mstore

MLoadMStore.thy
@@ -3,35 +3,49 @@ theory MLoadMStore
 begin
 
 type_synonym val    = nat
-type_synonym memory = "nat => val option"
+type_synonym memory = "val list"
 
 
 definition empty_memory :: memory where
-  "empty_memory _ = None"
+  "empty_memory = []"
 
-
-definition mstore :: "memory  =>  nat => val => memory" where
-  "mstore mem addr v = mem(addr := Some v)"
-
+definition mstore :: "memory => nat=> val=> memory" where
+  "mstore mem addr v =
+     (if addr < length mem
+      then list_update mem addr v
+      else mem @ replicate (addr - length mem) 0 @ [v])"
 
 definition mload :: "memory => nat => val option" where
-  "mload mem addr = mem addr"
+  "mload mem addr =
+     (if addr < length mem
+      then Some (mem ! addr)
+      else None)"
 
+(* Tests *)
 
-value "empty_memory 0"                         
-value "mload empty_memory 10"                
-value "mstore empty_memory 4 255 4"            
-value "mload (mstore empty_memory 4 255) 4"    
+value "empty_memory"
+  (* = [] *)
 
+value "mload empty_memory 10"
+  (* = None *)
 
+value "mstore empty_memory 4 255"
+  (* = [0, 0, 0, 0, 255] *)
 
+value "mload (mstore empty_memory 4 255) 4"
+  (* = Some 255 *)
+(*
+  mload XXX ....
+*)
 lemma test_mload_empty:
   "mload empty_memory 0 = None"
   by (simp add: mload_def empty_memory_def)
 
 lemma test_mstore_basic:
   "mload (mstore empty_memory 10 42) 10 = Some 42"
-  by (simp add: mload_def mstore_def empty_memory_def)
+  unfolding mload_def mstore_def empty_memory_def
+  by (simp add: nth_append)
+
 
 lemma test_mstore_other_addr_untouched:
   "mload (mstore empty_memory 5 99) 6 = None"
@@ -39,7 +53,9 @@ lemma test_mstore_other_addr_untouched:
 
 lemma test_mstore_multiple:
   "mload (mstore (mstore empty_memory 3 100) 4 200) 4 = Some 200"
-  by (simp add: mload_def mstore_def empty_memory_def)
+  unfolding mload_def mstore_def empty_memory_def
+  by (simp add: nth_append nth_list_update)
+
 
 lemma test_mstore_overwrite:
   "mload (mstore (mstore empty_memory 1 11) 1 22) 1 = Some 22"
@@ -47,14 +63,45 @@ lemma test_mstore_overwrite:
 
 lemma test_mstore_then_check_previous:
   "mload (mstore (mstore empty_memory 8 88) 9 99) 8 = Some 88"
-  by (simp add: mload_def mstore_def empty_memory_def)
+  unfolding mload_def mstore_def empty_memory_def
+  by (simp add: nth_append nth_list_update)
 
 lemma test_mstore_and_empty_check:
-  "mload (mstore empty_memory 7 77) 6 = None"
-  by (simp add: mload_def mstore_def empty_memory_def)
+  "mload (mstore empty_memory 7 77) 6 = Some 0"
+  unfolding mload_def mstore_def empty_memory_def
+  by (simp add: nth_append)
+
 
 lemma test_mstore_zero_addr:
   "mload (mstore empty_memory 0 1) 0 = Some 1"
   by (simp add: mload_def mstore_def empty_memory_def)
 
+
 end
+(*
+// SPDX-License-Identifier: MIT
+pragma solidity ^0.8.0;
+
+contract MemoryModel {
+    mapping(uint256 => uint256) private mem;
+    uint256 private maxIndex = 0;
+
+    function mstore(uint256 addr, uint256 v) public {
+        mem[addr] = v;
+        if (addr >= maxIndex) {
+            maxIndex = addr + 1;
+        }
+    }
+    
+    function mload(uint256 addr) public view returns (uint256) {
+        if (addr >= maxIndex) {
+            return type(uint256).max;
+        }
+        return mem[addr];
+    }
+    
+    
+    function isInitialized(uint256 addr) public view returns (bool) {
+        return addr < maxIndex;
+    }
+}*)
